fix: the MaxSum.v

algorithms/MaxSum.v
@@ -1,21 +1,25 @@
-Require Import Coq.Lists.List. 
-Require Import Coq.ZArith.ZArith. 
+Require Import Coq.Lists.List.
+Require Import Coq.ZArith.ZArith.
 Require Import Coq.Classes.Morphisms.
 Require Import Coq.Logic.Classical_Prop.
 Require Import Coq.micromega.Psatz.
 Require Import SetsClass.SetsClass.
-From MonadLib.SetMonad Require Import SetBasic SetHoare FixpointLib. 
-From MaxMinLib Require Import MaxMin Interface. 
+From MonadLib.SetMonad Require Import SetBasic SetHoare FixpointLib.
+From MaxMinLib Require Import MaxMin Interface.
 Require Import Algorithms.MapLib.
-From ListLib.Base Require Import Inductive Positional. 
-From ListLib.General Require Import Forall IndexedElements Length Presuffix. 
+From ListLib.Base Require Import Inductive Positional.
+From ListLib.General Require Import Forall IndexedElements Length Presuffix.
 
 Import ListNotations.
 Import MonadNotation.
-Local Open Scope monad. 
-Local Open Scope Z. 
+Local Open Scope monad.
+Local Open Scope Z.
 
-Definition max_sum (l:  list Z): program (Z * list Z) :=
+(* ========================================================================== *)
+(* 1. 原算法定义 *)
+(* ========================================================================== *)
+
+Definition max_sum (l: list Z): program (Z * list Z) :=
   '(max1, ans1, _, _) <- list_iter
                            (fun n =>
                               fun '(max1, ans1, max2, ans2) =>
@@ -28,21 +32,24 @@ Definition max_sum (l:  list Z): program (Z * list Z) :=
                            (0, [], 0, []);;
   ret (max1, ans1).
 
-(* Definition of non-adjacent indices: il is a list of indices *)
+(* ========================================================================== *)
+(* 2. 基础定义 *)
+(* ========================================================================== *)
+
 Definition non_adjacent_in (il: list Z): Prop :=
   sincr il /\ forall i j, In i il -> In j il -> i + 1 <> j.
 
-(* s is a non-adjacent subsequence of l, with index list il *)
-Definition non_adjacent_subseq (s l :  list Z): Prop:=
-  exists il, is_indexed_elements l il s /\ non_adjacent_in il. 
+Definition non_adjacent_subseq (s l : list Z): Prop :=
+  exists il, is_indexed_elements l il s /\ non_adjacent_in il.
 
-(* Definition of sum of a list *)
 Definition sum (l: list Z) : Z := fold_right Z.add 0 l.
 
-(* Definition of the feasible set *)
-Definition feasible_set (l :  list Z) (s : list Z) := non_adjacent_subseq s l.
+Definition feasible_set (l : list Z) (s : list Z) := non_adjacent_subseq s l.
 
-(* Maximum value of the set *)
+(* ========================================================================== *)
+(* 3. 规范定义 *)
+(* ========================================================================== *)
+
 Definition max_value_spec (l: list Z) (m: Z) : Prop :=
   (exists s,
       feasible_set l s /\
@@ -51,195 +58,124 @@ Definition max_value_spec (l: list Z) (m: Z) : Prop :=
   \/
   ((forall s, feasible_set l s -> sum s <= 0%Z) /\ m = 0%Z).
 
-(* Maximum value of the set excluding the last element *)
-Definition max_value_spec_excl_last (prefix:  list Z) (m: Z) : Prop :=
-  (exists s il,
-     is_indexed_elements prefix il s /\ non_adjacent_in il
-     /\ Forall (fun i => i < Zlength prefix - 1) il
-     /\ sum s = m
-     /\ forall t il', is_indexed_elements prefix il' t /\ non_adjacent_in il'
-                      /\ Forall (fun i => i < Zlength prefix - 1) il'
-                      -> sum t <= m)
-  \/
-  ((forall s il, is_indexed_elements prefix il s /\ non_adjacent_in il
-                 /\ Forall (fun i => i < Zlength prefix - 1) il
-                 -> sum s <= 0%Z)
-   /\ m = 0%Z).
+Definition max_sum_full_spec (l: list Z) (m: Z) (s: list Z) : Prop :=
+  max_value_spec l m /\
+  feasible_set l s /\
+  sum s = m.
 
-(* Invariant *)
-Definition P (prefix: list Z) (st: Z * list Z * Z * list Z) : Prop :=
-  let '(max1, ans1, max2, ans2) := st in
-  (exists il1, is_indexed_elements prefix il1 ans1 /\ non_adjacent_in il1)
-  /\ (exists il2, is_indexed_elements prefix il2 ans2 /\ non_adjacent_in il2
-                  /\ Forall (fun i => i < Zlength prefix - 1) il2)
-  /\ max_value_spec prefix max1
-  /\ max_value_spec_excl_last prefix max2. 
-
-(* Check if a list is strictly increasing *)
-Definition is_strictly_increasing (l: list Z) : Prop :=
-  forall i j, 0 <= i -> i < j -> j < Zlength l ->
-    exists vi vj, Znth_error l i = Some vi /\ 
-                  Znth_error l j = Some vj /\ 
-                  vi < vj.
-
-(* Check if a subsequence is an increasing subsequence *)
-Definition is_increasing_subseq (s l:  list Z) : Prop :=
-  is_subsequence l s /\ is_strictly_increasing s. 
-
-(* State for LIS algorithm: (last element, length, subsequence) *)
-Definition LIS_state := (Z * Z * list Z)%type.
-
-(* LIS Algorithm Definition *)
-Definition LIS (l: list Z) (least: Z): program (Z * list Z) :=
-  st <- list_iter
-    (fun n st =>
-      '(n0, len0, l0) <- max_object_of_subset
-        Z.le
-        (fun '(n0, len0, l0) => In (n0, len0, l0) st /\ n0 < n)
-        (fun '(n0, len0, l0) => len0);;
-      ret (st ++ [(n, len0 + 1, l0 ++ [n])]))
-    l
-    [(least, 0, [])];;
-  '(n0, len0, l0) <- max_object_of_subset
-    Z.le
-    (fun '(n0, len0, l0) => In (n0, len0, l0) st)
-    (fun '(n0, len0, l0) => len0);;
-  ret (len0, l0).
-
-(* Invariant for LIS Algorithm *)
-Definition LIS_invariant (prefix: list Z) (least: Z) (st: list LIS_state) : Prop :=
-  forall n len l,
-    In (n, len, l) st ->
-    is_increasing_subseq l prefix /\
-    (l = [] \/ Znth_error l (Zlength l - 1) = Some n) /\
-    Zlength l = len /\
-    (forall l', is_increasing_subseq l' prefix ->
-                (l' = [] \/ Znth_error l' (Zlength l' - 1) = Some n) ->
-                Zlength l' <= len).
-
-(* Specification for the length of the LIS *)
-Definition LIS_length_spec (l: list Z) (len: Z) : Prop :=
-  (exists s,
-    is_increasing_subseq s l /\
-    Zlength s = len /\
-    forall s', is_increasing_subseq s' l -> Zlength s' <= len).
-
-(* Full specification for LIS (including the sequence itself) *)
-Definition LIS_full_spec (l: list Z) (len: Z) (s: list Z) : Prop :=
-  is_increasing_subseq s l /\
-  Zlength s = len /\
-  forall s', is_increasing_subseq s' l -> Zlength s' <= len.
-
-(* Auxiliary Lemma: Length of a list is non-negative *)
-Lemma Zlength_nonneg_list : 
-  forall (l: list Z), 0 <= Zlength l. 
-Proof.
-  intros.  
-  apply Zlength_nonneg. 
+Lemma Zlength_nonneg_list : forall (l: list Z), 0 <= Zlength l.
+Proof. 
+  intros. 
+  apply Zlength_nonneg.
 Qed.
 
-(* Auxiliary Lemma: Empty list is a subsequence of any list *)
-Lemma is_subsequence_nil : forall (l : list Z), is_subsequence l [].
-Proof. 
+(* ========================================================================== *)
+(* 4. 难度任务 - 定理声明 *)
+(* ========================================================================== *)
+
+(* 第二档难度 *)
+Theorem max_sum_value_correct :
+  forall l,
+    Hoare (max_sum l)
+      (fun '(m, _) => max_value_spec l m).
+Proof.
 Admitted.
 
-(* Auxiliary Lemma: Empty list is increasing *)
-Lemma empty_is_increasing : 
-  forall l, is_increasing_subseq [] l.
+(* 第三档难度 *)
+Theorem max_sum_full_correct :
+  forall l,
+    Hoare (max_sum l)
+      (fun '(m, s) => max_sum_full_spec l m s).
 Proof.
-  intros l. 
-  split.
-  - apply is_subsequence_nil.
-  - unfold is_strictly_increasing. 
-    intros. 
-    unfold Zlength in *. 
-    simpl in *.          
-    lia.                
-Qed.
-
-(* Auxiliary Lemma: Appending an element preserves increasing property *)
-Lemma append_preserves_increasing :
-  forall l s n,
-    is_increasing_subseq s l ->
-    (s = [] \/ exists last, Znth_error s (Zlength s - 1) = Some last /\ last < n) ->
-    In n l ->
-    is_increasing_subseq (s ++ [n]) l.
-Proof. 
-Admitted.  (* Requires detailed proof *)
-
-(* Level 2: Prove LIS algorithm outputs the correct length *)
-Theorem LIS_length_correct :
-  forall l least,
-    least < fold_right Z.min (least - 1) l ->
-    Hoare (LIS l least)
-      (fun '(len, _) => LIS_length_spec l len).
-Proof.
-Admitted.  (* Main proof framework, requires induction on list_iter *)
-
-(* Level 3: Prove LIS algorithm outputs a correct subsequence *)
-Theorem LIS_full_correct :
-  forall l least,
-    least < fold_right Z.min (least - 1) l ->
-    Hoare (LIS l least)
-      (fun '(len, s) => LIS_full_spec l len s).
-Proof.
-Admitted. (* Based on length correctness, further prove sequence maximality *)
+Admitted.
 
 (* ========================================================================== *)
-(* Level 4: Lexicographically Minimal LIS *)
+(* 5. 第四档难度 - 字典序最小 *)
 (* ========================================================================== *)
 
-(* Lexicographical comparison of indices *)
+(* 字典序比较 *)
 Fixpoint index_lex_lt (il1 il2: list Z) : Prop :=
   match il1, il2 with
   | [], [] => False
-  | [], _ ::  _ => True
-  | _ ::  _, [] => False
+  | [], _ :: _ => True
+  | _ :: _, [] => False
   | i1 :: il1', i2 :: il2' =>
       i1 < i2 \/ (i1 = i2 /\ index_lex_lt il1' il2')
   end.
 
-(* Specification for Lexicographically Minimal LIS *)
-Definition LIS_lex_min_spec (l: list Z) (len: Z) (s: list Z) : Prop :=
-  exists il,
-    is_indexed_elements l il s /\
-    is_strictly_increasing s /\
-    Zlength s = len /\
-    (* s is the longest *)
-    (forall s', is_increasing_subseq s' l -> Zlength s' <= len) /\
-    (* The index sequence of s is lexicographically minimal *)
-    (forall s' il',
-      is_indexed_elements l il' s' ->
-      is_strictly_increasing s' ->
-      Zlength s' = len ->
-      index_lex_lt il il' \/ il = il').
+(* 字典序最小规范 *)
+Definition lex_min_spec (l: list Z) (m: Z) (s: list Z) (il: list Z) : Prop :=
+  max_sum_full_spec l m s /\
+  is_indexed_elements l il s /\
+  non_adjacent_in il /\
+  (forall s' il', 
+     feasible_set l s' -> 
+     is_indexed_elements l il' s' -> 
+     non_adjacent_in il' ->
+     sum s' = m -> 
+     index_lex_lt il il' \/ il = il').
 
-(* Modified LIS Algorithm (Prioritizes Lexicographically Minimal) *)
-Definition LIS_lex_min (l: list Z) (least: Z): program (Z * list Z) :=
-  st <- list_iter
-    (fun n st =>
-      res <- max_object_of_subset
-        Z.le
-        (fun '(n0, len0, l0, il0) =>
-          In (n0, len0, l0, il0) st /\ n0 < n)
-        (fun '(n0, len0, l0, il0) => len0);;
-      let '(n0, len0, l0, il0) := res in
-      (* Choose lexicographically minimal for same length *)
-      ret (st ++ [(n, len0 + 1, l0 ++ [n], il0 ++ [Zlength l0])]))
-    l
-    [(least, 0, [], [])];;
-  res <- max_object_of_subset
-    Z.le
-    (fun '(n0, len0, l0, il0) => In (n0, len0, l0, il0) st)
-    (fun '(n0, len0, l0, il0) => len0);;
-  let '(n0, len0, l0, il0) := res in
-  ret (len0, l0).
+(* 
+   修改后的算法：max_sum_lex
+   状态元组: (max1, ans1, il1, max2, ans2, il2, idx)
+   max1/ans1/il1: 当前最优解（和，序列，索引）
+   max2/ans2/il2: 不选前一个元素的最优解（和，序列，索引）
+   idx: 当前处理元素的索引
+*)
+Definition max_sum_lex (l: list Z): program (Z * list Z * list Z) :=
+  '(max1, ans1, il1, _, _, _, _) <- 
+    list_iter
+      (fun n =>
+         fun '(max1, ans1, il1, max2, ans2, il2, idx) =>
+           (* 方案1: 包含当前元素 n (前提是不包含前一个) -> 基础是从 (max2, ans2, il2) 转移而来 *)
+           let cand_inc_sum := max2 + n in
+           let cand_inc_ans := ans2 ++ [n] in
+           let cand_inc_il  := il2 ++ [idx] in
+           
+           (* 方案2: 不包含当前元素 n -> 基础是从 (max1, ans1, il1) 转移而来 *)
+           let cand_exc_sum := max1 in
+           let cand_exc_ans := ans1 in
+           let cand_exc_il  := il1 in
 
-(* Level 4: Prove modified algorithm outputs lexicographically minimal LIS *)
-Theorem LIS_lex_min_correct : 
-  forall l least,
-    least < fold_right Z.min (least - 1) l ->
-    Hoare (LIS_lex_min l least)
-      (fun '(len, s) => LIS_lex_min_spec l len s).
+           (* 新的 max2/ans2/il2 将会变成当前的 max1/ans1/il1 (为了下一次迭代做准备) *)
+           let next_max2 := max1 in
+           let next_ans2 := ans1 in
+           let next_il2  := il1 in
+           let next_idx  := idx + 1 in
+
+           (* 修复：嵌套 choice 以处理三个分支 *)
+           choice
+             (* Case 1: 包含当前元素使得和严格更大 *)
+             (assume (cand_inc_sum > cand_exc_sum);; 
+              ret (cand_inc_sum, cand_inc_ans, cand_inc_il, next_max2, next_ans2, next_il2, next_idx))
+             
+             (choice
+                (* Case 2: 不包含当前元素使得和严格更大 *)
+                (assume (cand_inc_sum < cand_exc_sum);;
+                 ret (cand_exc_sum, cand_exc_ans, cand_exc_il, next_max2, next_ans2, next_il2, next_idx))
+                
+                (* Case 3: 和相等，比较字典序 *)
+                (assume (cand_inc_sum = cand_exc_sum);;
+                  choice 
+                    (* 包含当前元素的索引序列字典序 更小 *)
+                    (assume (index_lex_lt cand_inc_il cand_exc_il);;
+                     ret (cand_inc_sum, cand_inc_ans, cand_inc_il, next_max2, next_ans2, next_il2, next_idx))
+                    
+                    (* 不包含当前元素的索引序列字典序 更小 或 相等 *)
+                    (* 如果字典序相等，通常优先选不包含的（因为较短），或者保持原样 *)
+                    (assume (~ index_lex_lt cand_inc_il cand_exc_il);;
+                     ret (cand_exc_sum, cand_exc_ans, cand_exc_il, next_max2, next_ans2, next_il2, next_idx))
+                )
+             )
+      )
+      l
+      (0, [], [], 0, [], [], 0);; (* 初始状态，索引从 0 开始 *)
+  ret (max1, ans1, il1).
+
+(* 第四档难度定理 *)
+Theorem max_sum_lex_correct :
+  forall l,
+    Hoare (max_sum_lex l)
+      (fun '(m, s, il) => lex_min_spec l m s il).
 Proof.
-Admitted. 
+Admitted.
